HOL/testItreeScript.sml
@@ -7,7 +7,7 @@
  * depending on context.
  *
  * In comparision to the clock approach in cakeML's FBS semantics, there is less
- * distinction between finite/infinite programs, which allows local reasoning.
+ * distinction between finite|infinite programs, which allows local reasoning.
  * Oracle queries are encoded by events, and 'evaluating' in a context where the
  * responses are limited, we can simulate interaction with the external world.
  * Although that possibility depends on the granularity of restrictions on results.
@@ -15,21 +15,22 @@
  * specifications should be *structural*, proofs should be *syntax-directed*
  *
  * One promising approach:
- * 1. express a clear (tauless) decomposition of the spec w/ conditions on FFI
+ * 1. express a clear (tauless) decomposition of the spec with conditions on FFI
  * 2. prove equivalence to the actual program semantics via weak bisimulation
  *
- * future work: ideally we want some way of automatically unfolding/executing a
+ * future work: ideally we want some way of automatically unfolding|executing a
  * program, to easily show facts about its interaction tree directly. This should
  * also allow for automated removal of Tau nodes. Could this be easier with types?
  *
  * note: Since they are the greatest fixpoint, they may also encode recursive tree
  * types using appropriate event data - e.g. W-trees. *
- * note: programs/simps/rewrites getting stuck in general is hard to predict and
- * annoying, proving strong normalization is the way out/weak ad-hoc size measure
+ * note: programs|simps|rewrites getting stuck in general is hard to predict and
+ * annoying, proving strong normalization is the way out|weak ad-hoc size measure
  * note: look into how to execute coinductive programs with progress?
  *)
 
-open HolKernel boolLib bossLib BasicProvers;
+open HolKernel boolLib bossLib BasicProvers; (* recommended by Magnus *)
+open stringLib; (* parsing, text examples etc. *)
 open itreeTauTheory;
 
 (* open monadsyntax; *)
@@ -62,15 +63,8 @@ val or4_tac = disj2_tac >> disj2_tac >> disj2_tac;
    where f = structure map (into primed itree), seed = itree algebra instance
  *)
 
-Theorem spin_unfold[simp]:
-  Tau spin = spin
-Proof
-  rw[spin, Once itree_unfold]
-QED
-
 (* echo taken from paper, a bit different with HOL unfold vs deptypes *)
 (* note: response types can't be restricted per event type *)
-
 Datatype:
   IO = Input | Output num
 End
@@ -111,8 +105,8 @@ Proof
   metis_tac[strip_tau_cases, itree_wbisim_cases]
 QED
 
-(*/
-  coinduction
+(*/ coinduction
+   for greater structural variation
  *)
 
 (* finite on all paths: generates backwards coind & forwards cases *)
@@ -135,14 +129,6 @@ Proof
   rw[Once itree_fin_cases]
 QED
 
-Theorem spin_inf:
-  itree_inf spin
-Proof
-  irule itree_inf_coind >>
-  qexists_tac ‘λt. t = (Tau t)’ >>
-  metis_tac[spin_unfold]
-QED
-
 Definition vis_spin_def:
   vis_spin = itree_unfold (λs. Vis' s I) 0
 End
@@ -157,13 +143,241 @@ QED
 
 (* looping vis nodes *)
 
-open arithmeticTheory;
-open stringLib;
-
 Definition iterate_def:
   iterate emit succ zero =
   itree_unfold (λs'. Vis' (emit s') (λ_. (succ s'))) zero
 End
+
+open panItreeSemTheory;
+
+(*/ equational theorems for mrec
+   mrec expresses a recursive computation by iterating Vis INL
+ *)
+
+(* iiter (Ret INL) → Tau (itree_unfold (iiter_cb (mrec_cb h_prog))
+                           (mrec_cb h_prog (bind (rh state_res) k))) to continue *)
+(* mrec: Vis (INL (prog × newstate)) k → Ret (INL (h_prog prog bind k)) *)
+(* mrec: Vis (INR (svis_ev × result->itree)) k → Ret (INL (h_prog prog bind k)) *)
+Definition mrec_cb_def[simp]:
+    mrec_cb rh (Ret r) = Ret (INR r)
+  ∧ mrec_cb rh (Tau t) = Ret (INL t)
+  ∧ mrec_cb rh (Vis (INL state_res) k) = Ret (INL (bind (rh state_res) k))
+  ∧ mrec_cb rh (Vis (INR   ffi_res) k) = Vis ffi_res (λx. Ret (INL (k x)))
+End
+
+Theorem itree_mrec_alt:
+  itree_mrec rh seed = iter (mrec_cb rh) (rh seed)
+Proof
+  rw[itree_mrec_def] >>
+  AP_THM_TAC >>
+  AP_TERM_TAC >>
+  rw[FUN_EQ_THM] >>
+  rw[DefnBase.one_line_ify NONE mrec_cb_def, combinTheory.o_DEF]
+QED
+
+Theorem iter_mrec_cb_thm[simp]:
+  iter (mrec_cb rh) (Ret x) = Ret x ∧
+  iter (mrec_cb rh) (Tau t) = Tau (iter (mrec_cb rh) t) ∧
+  iter (mrec_cb rh) (Vis (INL s) g) = Tau (iter (mrec_cb rh) (bind (rh s) g)) ∧
+  iter (mrec_cb rh) (Vis (INR e) k) = Vis e (λx. Tau (iter (mrec_cb rh) (k x)))
+Proof
+  rw[Once itree_iter_thm] >> rw[Once itree_iter_thm]
+QED
+
+Theorem mrec_cb_ret_inv:
+  mrec_cb rh t = Ret (INR r) ⇒ t = (Ret r)
+Proof
+  rw[DefnBase.one_line_ify NONE mrec_cb_def] >>
+  Cases_on ‘t’ >> fs[] >-
+   (Cases_on ‘a’ >> fs[])
+QED
+
+Theorem itree_bind_ret_inv:
+  bind t k = Ret r ⇒ ∃r'. t = Ret r' ∧ Ret r = (k r')
+Proof
+  Cases_on ‘t’ >> fs[itree_bind_thm]
+QED
+
+(* mrec iterates sequentially on its seed *)
+Theorem itree_mrec_bind:
+  iter (mrec_cb rh) (bind t k) =
+  bind (iter (mrec_cb rh) t) (λx. iter (mrec_cb rh) (k x))
+Proof
+  rw[Once itree_strong_bisimulation] >>
+  qexists_tac ‘λa b. ∃ps. a = iter (mrec_cb rh) (bind ps k) ∧
+                          b = bind (iter (mrec_cb rh) ps)
+                                (λx. iter (mrec_cb rh) (k x))’ >>
+  rw[] >-
+   (metis_tac[]) >-
+   (‘bind (mrec_cb rh (bind ps k))
+       (λx. case x of INL a => Tau (iter (mrec_cb rh) a) | INR b => Ret b)
+     = Ret x’
+      by gvs[Once itree_iter_thm] >>
+    qpat_x_assum ‘Ret x = iter _ _’ kall_tac >>
+    drule itree_bind_ret_inv >> pop_assum kall_tac >> strip_tac >>
+    Cases_on ‘r'’ >> gvs[] >>
+    drule mrec_cb_ret_inv >> strip_tac >>
+    drule itree_bind_ret_inv >> strip_tac >>
+    fs[Once itree_iter_thm] >>
+    fs[Once itree_iter_thm]) >-
+   (Cases_on ‘ps’ >-
+     (fs[] >> metis_tac[]) >-
+     (fs[] >> metis_tac[]) >-
+     (Cases_on ‘a’ >> fs[] >-
+       (fs[GSYM itree_bind_assoc] >> metis_tac[]))) >-
+   (Cases_on ‘ps’ >> fs[] >-
+     (metis_tac[]) >-
+     (Cases_on ‘a'’ >> fs[] >>
+      strip_tac >> disj1_tac >>
+      qexists_tac ‘Tau (g s)’ >>
+      rw[]))
+QED
+
+(*/ pancake theorems
+   syntax directed rewrites TODO figure out how to lift these to FFItree
+ *)
+
+Theorem seq_thm:
+  itree_mrec h_prog (Seq p p2, s) =
+  Tau (bind (itree_mrec h_prog (p, s))
+            (λ(res,s').
+               if res = NONE
+               then Tau (itree_mrec h_prog (p2, s'))
+               else (Ret (res, s'))))
+Proof
+  rw[itree_mrec_alt] >>
+  rw[h_prog_def, h_prog_rule_seq_def] >>
+  rw[itree_mrec_bind] >>
+  AP_TERM_TAC >>
+  rw[FUN_EQ_THM] >>
+  Cases_on ‘x’ >> rw[]
+QED
+
+Definition revert_binding_def:
+  revert_binding name old_s
+  = (λ(res,s').
+       Ret
+       (res,
+        s' with locals :=
+        res_var s'.locals (name,FLOOKUP old_s.locals name)))
+End
+
+Theorem h_prog_rule_dec_alt:
+  h_prog_rule_dec vname e p s =
+  case eval s e of
+    NONE => Ret (SOME Error,s)
+  | SOME value =>
+      Vis (INL (p,s with locals := s.locals |+ (vname,value)))
+          (revert_binding vname s)
+Proof
+  rw[h_prog_rule_dec_def, revert_binding_def]
+QED
+
+(* f, f' type vars instantiated differently smh *)
+(* relies on mrec_cb h_prog rev -> only Ret INR, so can't prolong iteration *)
+Theorem itree_mrec_bind_ret:
+  ∀f f'.
+    (∀a. ∃r. (f a) = (Ret r) ∧ (f' a) = (Ret r)) ⇒
+    ∀t. iter (mrec_cb h_prog) (bind t f) = (bind (iter (mrec_cb h_prog) t) f')
+Proof
+  rpt strip_tac >>
+  rw[itree_mrec_bind] >>
+  AP_TERM_TAC >> rw[FUN_EQ_THM] >>
+  pop_assum $ qspec_then ‘x’ strip_assume_tac >> fs[]
+QED
+
+Theorem dec_thm:
+  (eval s e = SOME k) ⇒
+  (itree_mrec h_prog (Dec name e p,s))
+  = Tau (bind
+         (itree_mrec h_prog (p,s with locals := s.locals |+ (name,k)))
+         (revert_binding name s))
+Proof
+  rw[itree_mrec_alt] >>
+  rw[h_prog_def, h_prog_rule_dec_def] >>
+  rw[GSYM revert_binding_def] >>
+  irule itree_mrec_bind_ret >>
+  rw[revert_binding_def] >>
+  Cases_on ‘a’ >> rw[]
+QED
+
+(*/ massaging into FFItree
+   fix merged!
+ *)
+
+Definition massage_cb_def[simp]:
+  massage_cb (Ret (res, s)) = Ret' res ∧
+  massage_cb (Tau kt) = Tau' kt ∧
+  massage_cb (Vis (svis_ev, scb) st) = Vis' svis_ev (λffi_res. st (scb ffi_res))
+End
+
+(* massage Ret type from (η x state) -> η *)
+(* convert Vis (sem_vis_event x (FFI_result -> itree)) ((prog x state) -> %itree)
+-> Vis sem_vis_event (FFI_result -> itree) *)
+Definition to_ffi_def:
+  to_ffi t = itree_unfold massage_cb t
+End
+
+Theorem to_ffi_alt[simp]:
+  to_ffi (Tau t) = Tau (to_ffi t) ∧
+  to_ffi (Ret (p,s)) = Ret p ∧
+  to_ffi (Vis (svis_ev,scb) g) = Vis svis_ev (λffi_res. to_ffi (g (scb (ffi_res))))
+Proof
+  rw[to_ffi_def] >> rw[Once itree_unfold] >>
+  rw[combinTheory.o_DEF]
+QED
+
+Theorem pull_ffi_case[simp]:
+  (to_ffi
+   (iter (mrec_cb h_prog)
+         (f (case res of
+               FFI_return new_ffi new_bytes => a new_ffi new_bytes
+             | FFI_final outcome => b outcome))))
+  =
+  (case res of
+     FFI_final outcome =>
+       to_ffi (iter (mrec_cb h_prog) (f (b outcome)))
+   | FFI_return new_ffi new_bytes =>
+       to_ffi (iter (mrec_cb h_prog) (f (a new_ffi new_bytes))))
+Proof
+  rw[FUN_EQ_THM] >>
+  Cases_on ‘res’ >> rw[]
+QED
+
+(* TODO no higher order unification? *)
+Theorem pull_ffi_case2[simp]:
+  (to_ffi
+   (f (case res of
+         FFI_return new_ffi new_bytes => a new_ffi new_bytes
+       | FFI_final outcome => b outcome)))
+  =
+  (case res of
+     FFI_final outcome => to_ffi (f (b outcome))
+   | FFI_return new_ffi new_bytes => to_ffi (f (a new_ffi new_bytes)))
+Proof
+  rw[FUN_EQ_THM] >>
+  Cases_on ‘res’ >> rw[]
+QED
+
+Theorem itree_evaluate_alt:
+  itree_evaluate p s = to_ffi (itree_mrec h_prog (p,s))
+Proof
+  rw[itree_evaluate_def, to_ffi_def] >>
+  AP_THM_TAC >> (* same fn => same on same arg, backwards *)
+  AP_TERM_TAC >>
+  rw[FUN_EQ_THM] >>
+  rw[DefnBase.one_line_ify NONE massage_cb_def, combinTheory.o_DEF]
+QED
+
+
+
+
+
+
+(*/ testing recursive specifications
+   TODO preludes and postludes, how to lift??
+ *)
+open arithmeticTheory;
 
 Definition even_spec_def:
   even_spec k = iterate (λx. if EVEN x then "even" else "odd") (λn. 1 + n) k
@@ -254,3 +468,82 @@ End
 (* Proof *)
 (*   cheat *)
 (* QED *)
+
+(*/ interp nonsense
+   weird
+ *)
+
+Definition interp_cb_def[simp]:
+  interp_cb rh (Ret r) = Ret (INR r) ∧
+  interp_cb rh (Tau t) = Ret (INL t) ∧
+  interp_cb rh (Vis e k) = bind (rh e) (λa. Ret (INL (k a)))
+End
+
+(* (E -> itree E' R) -> itree E R -> itree E' R *)
+Definition itree_interp_def:
+  itree_interp rh it = itree_iter (interp_cb rh) it
+End
+
+Theorem interp_cb_ret_inv:
+  interp_cb rh t = Ret (INR r) ⇒ t = (Ret r)
+Proof
+  rw[DefnBase.one_line_ify NONE interp_cb_def] >>
+  Cases_on ‘t’ >> fs[] >>
+  Cases_on ‘rh a’ >> fs[]
+QED
+
+Theorem itree_interp_ret:
+  itree_interp rh (Ret r) = Ret r
+Proof
+  rw[itree_interp_def] >>
+  rw[Once itree_iter_thm]
+QED
+
+Theorem itree_interp_trigger:
+  itree_interp rh (Vis e Ret) ≈ rh e
+Proof
+  rw[itree_interp_def] >>
+  rw[Once itree_iter_thm] >>
+  rw[itree_bind_assoc] >>
+  rw[Once itree_iter_thm] >>
+  irule itree_wbisim_coind >>
+  qexists_tac ‘λa b. ∃t. a = bind t (λa. Tau (Ret a)) ∧ b = t’ >>
+  rw[] >>
+  Cases_on ‘a1’ >> rw[]
+QED
+
+Theorem itree_interp_bind:
+  itree_interp rh (bind t k) = bind (itree_interp rh t) (λr. itree_interp rh (k r))
+Proof
+  rw[itree_interp_def] >>
+  rw[Once itree_strong_bisimulation] >>
+  qexists_tac ‘λa b. ∃ps. a = iter (interp_cb rh) (bind ps k) ∧
+                          b = bind (iter (interp_cb rh) ps)
+                                   (λx. iter (interp_cb rh) (k x))’ >>
+  rw[] >-
+   (metis_tac[])
+   (cheat
+   )
+QED
+
+(* they are only weakly bisimilar *)
+Theorem itree_mrec_interp:
+  iter (mrec_cb rh) t ≈
+  itree_interp (λe. case e of
+                      (INL a) => (itree_mrec rh a)
+                    | (INR e) => Vis e Ret)
+  t
+Proof
+  rw[Once itree_mrec_alt, itree_interp_def] >>
+  rw[Once itree_iter_thm] >>
+  CONV_TAC $ RHS_CONV $ ONCE_REWRITE_CONV[itree_iter_thm] >>
+  Cases_on ‘e’ >> rw[] >-
+   (rw[itree_bind_assoc] >>
+    rw[itree_mrec_bind] >>
+    rw[GSYM itree_mrec_alt] >>
+    cheat
+   ) >-
+   (rw[FUN_EQ_THM] >>
+    rw[]
+   )
+QED
